-

Nsring.v
@@ -55,9 +55,37 @@ Compute (15 / 3)%nat.
 
 (* ℤn = ℤ/nℤ *)
 
-Definition Zn n := {a : nat | a <? S (S (n - 2)) = true}.
+Definition at_least_2 n := S (S (n - 2)).
 
-Theorem Zn_op_prop n r : r mod S (S (n - 2)) <? S (S (n - 2)) = true.
+Definition Zn n := {a : nat | a <? at_least_2 n = true}.
+
+Fixpoint prime_test cnt n d :=
+  match cnt with
+  | 0 => true
+  | S c =>
+      match n mod d with
+      | 0 => n <=? d
+      | S _ => prime_test c n (d + 1)
+      end
+  end.
+
+Definition is_prime n :=
+  match n with
+  | 0 | 1 => false
+  | S (S c) => prime_test c n 2
+  end.
+
+Fixpoint inv_mod_loop a n b :=
+  match b with
+  | 0 => 0
+  | S b' =>
+      if Nat.eq_dec (a * b' mod n) 1 then b'
+      else inv_mod_loop a n b'
+  end.
+
+Definition inv_mod a n := inv_mod_loop a n n.
+
+Theorem Zn_op_prop n r : r mod at_least_2 n <? at_least_2 n = true.
 Proof.
 intros.
 apply Nat.ltb_lt.
@@ -65,20 +93,20 @@ now apply Nat.mod_upper_bound.
 Qed.
 
 Definition Zn_v n v : Zn n :=
-  exist _ (v mod S (S (n - 2))) (Zn_op_prop n v).
+  exist _ (v mod at_least_2 n) (Zn_op_prop n v).
 
 Definition Zn_add n (a b : Zn n) : Zn n :=
   let r := proj1_sig a + proj1_sig b in
-  exist _ (r mod S (S (n - 2))) (Zn_op_prop n r).
+  exist _ (r mod at_least_2 n) (Zn_op_prop n r).
 Definition Zn_mul n (a b : Zn n) : Zn n :=
   let r := proj1_sig a * proj1_sig b in
-  exist _ (r mod S (S (n - 2))) (Zn_op_prop n r).
+  exist _ (r mod at_least_2 n) (Zn_op_prop n r).
 Definition Zn_opp n (a : Zn n) : Zn n :=
-  let r := S (S (n - 2)) - proj1_sig a in
-  exist _ (r mod S (S (n - 2))) (Zn_op_prop n r).
-Definition phony_Zn_inv n (a : Zn n) : Zn n :=
-  let r := 0 in
-  exist _ (r mod S (S (n - 2))) (Zn_op_prop n r).
+  let r := at_least_2 n - proj1_sig a in
+  exist _ (r mod at_least_2 n) (Zn_op_prop n r).
+Definition Zn_inv n (a : Zn n) : Zn n :=
+  let r := inv_mod (proj1_sig a) n in
+  exist _ (r mod at_least_2 n) (Zn_op_prop n r).
 
 Definition Zn_ring_like_op n : ring_like_op (Zn n) :=
   {| rngl_zero := Zn_v n 0;
@@ -86,7 +114,7 @@ Definition Zn_ring_like_op n : ring_like_op (Zn n) :=
      rngl_add := Zn_add n;
      rngl_mul := Zn_mul n;
      rngl_opp := Zn_opp n;
-     rngl_inv := phony_Zn_inv n |}.
+     rngl_inv := Zn_inv n |}.
 
 Theorem Zn_eq : ∀ n (a b : Zn n), proj1_sig a = proj1_sig b → a = b.
 Proof.
@@ -217,10 +245,61 @@ destruct (Nat.eq_dec a b) as [Hab| Hab]; [ left | right ]. {
 }
 Qed.
 
+Theorem prime_mul_inv_l_mod : ∀ n a,
+  is_prime n = true
+  → a ≠ 0
+  → (inv_mod a n * a) mod n = 1.
+Proof.
+intros * Hn Haz.
+...
+
+Theorem Zn_opt_mul_inv_l :
+  if is_prime n then ∀ a : Zn n, a ≠ 0%F → (¹/ a * a)%F = 1%F else True.
+Proof.
+intros.
+remember (is_prime n) as p eqn:Hp.
+symmetry in Hp.
+destruct p; [ | easy ].
+intros * Haz.
+destruct (lt_dec n 2) as [Hn2| Hn2]. {
+  destruct n; [ easy | ].
+  destruct n0; [ easy | ].
+  do 2 apply Nat.succ_lt_mono in Hn2.
+  easy.
+}
+apply Nat.nlt_ge in Hn2; cbn.
+apply Zn_eq; cbn - [ "mod" ].
+rewrite (Nat.mod_small 1). 2: {
+  apply -> Nat.succ_lt_mono.
+  apply Nat.lt_0_succ.
+}
+rewrite Nat.mul_mod_idemp_l; [ | easy ].
+replace (at_least_2 n) with n. 2: {
+  destruct n as [| n']; [ easy | ].
+  destruct n'; [ easy | ].
+  unfold at_least_2.
+  do 2 rewrite Nat.sub_succ.
+  now rewrite Nat.sub_0_r.
+}
+...
+apply prime_mul_inv_l_mod; [ easy | ].
+destruct a as (a, Ha); cbn.
+cbn in Haz.
+intros H; apply Haz; clear Haz; subst a.
+apply Zn_eq; cbn; symmetry.
+apply Nat.sub_diag.
+Qed.
+
+Theorem Zn_opt_mul_inv_r :
+  if (is_prime n && negb true)%bool then ∀ a : Zn n, a ≠ 0%F → (a / a)%F = 1%F
+  else True.
+Proof.
+...
+
 Definition Zn_ring_like_prop : ring_like_prop (Zn n) :=
   {| rngl_is_comm := true;
      rngl_has_opp := true;
-     rngl_has_inv := false; (* except if n is prime *)
+     rngl_has_inv := is_prime n;
      rngl_has_dec_eq := true;
      rngl_is_domain := false;
      rngl_add_comm := Zn_add_comm;
@@ -236,8 +315,8 @@ Definition Zn_ring_like_prop : ring_like_prop (Zn n) :=
      rngl_opt_add_opp_l := Zn_add_opp_l;
      rngl_opt_mul_0_l := I;
      rngl_opt_mul_0_r := I;
-     rngl_opt_mul_inv_l := I;
-     rngl_opt_mul_inv_r := I;
+     rngl_opt_mul_inv_l := Zn_opt_mul_inv_l;
+     rngl_opt_mul_inv_r := Zn_opt_mul_inv_r;
      rngl_opt_eq_dec := Zn_eq_dec;
      rngl_opt_is_integral := I |}.
 
